feat: added fee to oracle

Oracle2/Oracle2.fst
@@ -3,6 +3,7 @@ module Oracle2
 open Zen.Base
 open Zen.Cost
 open Zen.Types
+open Zen.Data
 
 module CR = Zen.ContractResult
 module Dict = Zen.Dictionary
@@ -11,10 +12,15 @@ module RT = Zen.ResultT
 module Sha3 = Zen.Hash.Sha3
 module TX = Zen.TxSkeleton
 module W = Zen.Wallet
+module U64 = FStar.UInt64
+module Asset = Zen.Asset
+
 
 type commitData =
     { commit       : hash
     ; oraclePubKey : publicKey
+    ; feeAsset     : asset
+    ; feeAmount    : option U64.t
     }
 
 type attestData =
@@ -66,22 +72,47 @@ let hashCPK cpk = // 6
 -------------------------------------------------------------------------------
 *)
 
-val parseCommitData : publicKey -> option data -> commitData `RT.t` 81
-let parseCommitData sender msgBody = // 17
-    begin match msgBody with
-    | Some (Collection (Dict dict)) ->
-        let! commit = Dict.tryFind "Commit" dict in // 64
-        begin match commit with
-        | Some (Hash commit) ->
-            { commit       = commit
-            ; oraclePubKey = sender
-            } |> RT.ok
-        | _ ->
-            RT.failw "Could not parse Commit"
-        end
-    | _ ->
-        RT.autoFailw "MessageBody must be a dictionary."
-    end
+val parseDict: option data -> result (Dict.t data) `cost` 12
+let parseDict data = // 8
+    match data with
+    | Some data ->
+        data
+        |> tryDict // 4
+        |> RT.ofOptionT "Data parsing failed - the message body isn't a dictionary"
+    | None ->
+        RT.incFailw 4 "Data parsing failed - the message body is empty"
+
+val parseFeeAsset : Dict.t data -> asset `cost` 145
+let parseFeeAsset dict  = // 10
+    Dict.tryFind "FeeAsset" dict // 64
+    >?= tryString // 2
+    >?= Asset.parse // 64
+    >>= OT.maybeT Asset.zenAsset ret // 5
+
+val parseFeeAmount : Dict.t data -> option U64.t `cost` 70
+let parseFeeAmount dict = // 4
+    Dict.tryFind "FeeAmount" dict // 64
+    >?= tryU64 // 2
+
+val parseCommit : Dict.t data -> result hash `cost` 73
+let parseCommit dict = // 7
+    Dict.tryFind "Commit" dict // 64
+    >?= tryHash // 2
+    |> RT.ofOptionT "Could not parse Commit"
+
+val parseCommitData : publicKey -> option data -> commitData `RT.t` 318
+let parseCommitData sender msgBody = // (3 + 3 + 12)
+    let open RT in
+    parseDict msgBody >>= (fun dict   -> // 12
+    parseCommit dict  >>= (fun commit -> // 73
+        let! feeAsset  = parseFeeAsset  dict in // 145
+        let! feeAmount = parseFeeAmount dict in // 70
+        { commit       = commit
+        ; oraclePubKey = sender
+        ; feeAsset     = feeAsset
+        ; feeAmount    = feeAmount
+        } |> ret
+    ))
 
 val senderToLock : sender -> lock `OT.t` 551
 let senderToLock sender = // 15
@@ -100,13 +131,15 @@ let senderToLock sender = // 15
         |> incRet 536
     end
 
-val parseAttestData : sender -> option data -> attestData `RT.t` 790
-let parseAttestData sender msgBody = // 47
+val parseAttestData : sender -> option data -> attestData `RT.t` 1013
+let parseAttestData sender msgBody = // 55
     begin match msgBody with
     | Some (Collection (Dict dict)) ->
         let! commit       = Dict.tryFind "Commit"       dict in // 64
         let! oraclePubKey = Dict.tryFind "OraclePubKey" dict in // 64
         let! recipient    = Dict.tryFind "Recipient"    dict in // 64
+        let! feeAsset     = parseFeeAsset               dict in // 145
+        let! feeAmount    = parseFeeAmount              dict in // 70
         let! senderLock   = senderToLock sender              in // 551
         begin match commit with
         | Some (Hash commit) ->
@@ -117,6 +150,8 @@ let parseAttestData sender msgBody = // 47
                     { commitData =
                         { commit       = commit
                         ; oraclePubKey = pk
+                        ; feeAsset     = feeAsset
+                        ; feeAmount    = feeAmount
                         }
                     ; recipient = recip
                     } |> RT.ok
@@ -128,6 +163,8 @@ let parseAttestData sender msgBody = // 47
                         { commitData =
                             { commit       = commit
                             ; oraclePubKey = pk
+                            ; feeAsset     = feeAsset
+                            ; feeAmount    = feeAmount
                             }
                         ; recipient = lock
                         } |> RT.ok
@@ -156,23 +193,43 @@ let parseAttestData sender msgBody = // 47
 -------------------------------------------------------------------------------
 *)
 
-val hashCommitData : commitData -> hash `cost` 736
-let hashCommitData data = // 14
+val hashCommitData : commitData -> hash `cost` 1179
+let hashCommitData data = // 25
+    let! cpk = compress data.oraclePubKey in // 305
+    match data.feeAmount with
+    | None ->
+        ret Sha3.empty
+        >>= Sha3.updateHash data.commit // 192
+        >>= updateCPK cpk               // 205
+        >>= Sha3.finalize               // 20
+        |> inc 432
+    | Some amount ->
+        ret Sha3.empty
+        >>= Sha3.updateHash data.commit    // 192
+        >>= updateCPK cpk                  // 205
+        >>= Sha3.updateAsset data.feeAsset // 384
+        >>= Sha3.updateU64 amount          // 48
+        >>= Sha3.finalize                  // 20
+
+val hashAttestData : commitData -> hash `cost` 736
+let hashAttestData data = // 14
     let! cpk = compress data.oraclePubKey in // 305
     ret Sha3.empty
     >>= Sha3.updateHash data.commit // 192
     >>= updateCPK cpk               // 205
     >>= Sha3.finalize               // 20
 
-val mkAssets : contractId -> commitData -> assets `cost` 968
-let mkAssets (v, h) data = // 20
-    let! dataHash =
-        hashCommitData data in // 736
-    let! dataHash2 =
+val mkAssets : contractId -> commitData -> assets `cost` 2150
+let mkAssets (v, h) data = // 23
+    let! commitHash =
+        hashCommitData data in // 1179
+    let! attestHash1 = 
+        hashAttestData data in // 736
+    let! attestHash2 =
         ret Sha3.empty
-        >>= Sha3.updateHash dataHash // 192
-        >>= Sha3.finalize in         // 20
-    ret ({ commitment=v,h,dataHash; attestation=v,h,dataHash2 })
+        >>= Sha3.updateHash attestHash1 // 192
+        >>= Sha3.finalize in            // 20
+    ret ({ commitment=v,h,commitHash; attestation=v,h,attestHash2 })
 
 
 
@@ -186,9 +243,9 @@ val dataCommit :
     txSkeleton
     -> contractId
     -> commitData
-    -> txSkeleton `cost` 1110
+    -> txSkeleton `cost` 2292
 let dataCommit txSkel cid args = // 14
-    let! ({commitment = commitment}) = mkAssets cid args in // 968
+    let! ({commitment = commitment}) = mkAssets cid args in // 2150
     ret txSkel
     >>= TX.mint 1UL commitment               // 64
     >>= TX.lockToContract commitment 1UL cid // 64
@@ -198,18 +255,18 @@ val commit :
   -> sender
   -> option data
   -> txSkeleton
-  -> CR.t `cost` 1210
+  -> CR.t `cost` 2629
 let commit cid sender msgBody txSkel = // 16
     let open RT in
     let! tx =
         begin match sender with
         | PK pk ->
             ret msgBody
-            >>= parseCommitData pk                  // 81
-            >>= (liftCost << dataCommit txSkel cid) // 1110
+            >>= parseCommitData pk                  // 318
+            >>= (liftCost << dataCommit txSkel cid) // 2292
         | _ ->
             "Sender must be a public key"
-            |> RT.incFailw 1191
+            |> RT.incFailw 2610
         end
     in CR.ofResultTxSkel tx // 3
 
@@ -225,27 +282,35 @@ val attestTx :
     assets
     -> contractId
     -> (w : wallet)
-    -> lock
+    -> attestData
     -> txSkeleton
-    -> txSkeleton `OT.t` (128 + (W.size w * 128 + 192) + 64 + 31)
-let attestTx assets cid (w : wallet) (recipient : lock) txSkel = // 31
+    -> txSkeleton `OT.t` (0 + 64 + 64 + (Zen.Wallet.size w * 128 + 192) + 64 + 610 + 48)
+let attestTx assets cid (w : wallet) (data : attestData) txSkel = // 48
     let open OT in
     ret txSkel
     >>= (liftCost << TX.mint 1UL assets.attestation) // 64
-    >>= (liftCost << TX.lockToAddress assets.attestation 1UL recipient) // 64
+    >>= (liftCost << TX.lockToAddress assets.attestation 1UL data.recipient) // 64
     >>= TX.fromWallet assets.commitment 1UL cid w // W.size w * 128 + 192
     >>= (liftCost << TX.lockToContract assets.commitment 1UL cid) // 64
+    >>= begin match data.commitData.feeAmount with
+        | Some amount ->
+            TX.lockToPublicKey data.commitData.feeAsset amount data.commitData.oraclePubKey // 610
+            >> liftCost
+        | None ->
+            incRet 610
+            >> liftCost
+        end
 
 val dataAttest' :
     contractId
     -> (w : wallet)
     -> txSkeleton
     -> attestData
-    -> txSkeleton `RT.t` (968 + (0 + (128 + (W.size w * 128 + 192) + 64 + 31) + 0) + 16)
-let dataAttest' cid w txSkel args = // 16
-    let! assets = mkAssets cid args.commitData in // 968
+    -> txSkeleton `RT.t` (2150 + (0 + (0 + 64 + 64 + (W.size w * 128 + 192) + 64 + 610 + 48) + 0) + 15)
+let dataAttest' cid w txSkel data = // 16
+    let! assets = mkAssets cid data.commitData in // 2150
     ret txSkel
-    >>= attestTx assets cid w args.recipient
+    >>= attestTx assets cid w data // ...
     >>= RT.ofOption "Could not spend from wallet"
 
 val dataAttest :
@@ -253,10 +318,10 @@ val dataAttest :
     -> (w : wallet)
     -> txSkeleton
     -> attestData
-    -> txSkeleton `RT.t` (W.size w * 128 + 1405)
-let dataAttest cid w txSkel args = // 16
-    dataAttest' cid w txSkel args
-    |> (fun x -> x <: txSkeleton `RT.t` (W.size w * 128 + 1399))
+    -> txSkeleton `RT.t` (W.size w * 128 + 3213)
+let dataAttest cid w txSkel data = // 6
+    dataAttest' cid w txSkel data
+    |> (fun x -> x <: txSkeleton `RT.t` (W.size w * 128 + 3207))
 
 val attest :
     contractId ->
@@ -264,12 +329,12 @@ val attest :
     sender ->
     option data ->
     txSkeleton ->
-    CR.t `cost` (W.size w * 128 + 2208)
+    CR.t `cost` (W.size w * 128 + 4239)
 let attest cid w sender msgBody txSkel = // 10
     let open RT in
     let! tx =
-        parseAttestData sender msgBody // 790
-        >>= dataAttest cid w txSkel // W.size w * 128 + 1405
+        parseAttestData sender msgBody // 1013
+        >>= dataAttest cid w txSkel // W.size w * 128 + 3213
     in CR.ofResultTxSkel tx // 3
 
 
@@ -291,22 +356,22 @@ val main :
     -> state   : option data
     -> CR.t `cost`
         begin match command with
-        | "Commit" -> 1218
-        | "Attest" -> W.size w * 128 + 2216
+        | "Commit" -> 2637
+        | "Attest" -> W.size w * 128 + 4247
         | _        -> 8
         end
 let main txSkel _ cid command sender msgBody w _ = // 8
     begin match command with
     | "Commit" ->
-        commit cid sender msgBody txSkel // 1210
+        commit cid sender msgBody txSkel // 2629
         <: CR.t `cost`
             begin match command with
-            | "Commit" -> 1210
-            | "Attest" -> W.size w * 128 + 2208
+            | "Commit" -> 2629
+            | "Attest" -> W.size w * 128 + 4239
             | _        -> 0
             end
     | "Attest" ->
-        attest cid w sender msgBody txSkel // W.size w * 128 + 2208
+        attest cid w sender msgBody txSkel // W.size w * 128 + 4239
     | _ ->
         RT.failw "Command not recognized"
     end
@@ -322,8 +387,8 @@ val cf :
     -> nat `cost` 10
 let cf _ _ command _ _ w _ = // 10
     begin match command with
-    | "Commit" -> 1218
-    | "Attest" -> W.size w * 128 + 2216
+    | "Commit" -> 2637
+    | "Attest" -> W.size w * 128 + 4247
     | _        -> 8
     end
     |> ret
